working/composition/event_based_refinement/load_balancer/service_correspondence/multiplication_service/RefinementProof.v.dfy
@@ -1,21 +1,21 @@
 include "RefinementObligation.t.dfy"
 
 module RefinementProof refines RefinementTheorem {
-    ghost function ConstantsAbstraction(c: Constants) : Service.Constants
+    ghost function ConstantsAbstraction(c: Constants) : Spec.Constants
         //requires c.WF()
     {
-        Service.Constants
+        Spec.Constants
     }
 
-    ghost function VariablesAbstraction(c: Constants, v: Variables) : Service.Variables
+    ghost function VariablesAbstraction(c: Constants, v: Variables) : Spec.Variables
         //requires v.WF(c)
     {
-        Service.Variables(v.multSvc.hosts[0].requests, v.multSvc.hosts[0].replies)
+        Spec.Variables(v.multSvc.hosts[0].requests, v.multSvc.hosts[0].replies)
     }
 
     lemma {:axiom} UniqueParsingAxiom(pkt: seq<byte>)
-        ensures Service.ParseServiceReply(pkt).Some? || Service.ParseServiceRequest(pkt).Some? ==> AddSvc.ParseServiceReply(pkt).None? && AddSvc.ParseServiceRequest(pkt).None?
-        ensures AddSvc.ParseServiceReply(pkt).Some? || AddSvc.ParseServiceRequest(pkt).Some? ==> Service.ParseServiceReply(pkt).None? && Service.ParseServiceRequest(pkt).None?
+        ensures Spec.ParseServiceReply(pkt).Some? || Spec.ParseServiceRequest(pkt).Some? ==> AddSM.ParseServiceReply(pkt).None? && AddSM.ParseServiceRequest(pkt).None?
+        ensures AddSM.ParseServiceReply(pkt).Some? || AddSM.ParseServiceRequest(pkt).Some? ==> Spec.ParseServiceReply(pkt).None? && Spec.ParseServiceRequest(pkt).None?
 
     /// invariant tying network state to protocol state
     // can this be generalized and baked into the system model?
@@ -24,15 +24,15 @@ module RefinementProof refines RefinementTheorem {
     {
         && (forall pkt: Message<seq<byte>> :: 
             && pkt in v.network.sentMsgs
-            && Service.ParseServiceReply(pkt.msg).Some?
+            && Spec.ParseServiceReply(pkt.msg).Some?
             && pkt.src == c.multSvc.hosts[0].idSelf ==>
-                exists request: Message<Service.ServiceRequest> :: 
-                && Message(pkt.src, pkt.dest, Service.ParseServiceReply(pkt.msg).value) in v.multSvc.hosts[0].replies
+                exists request: Message<Spec.ServiceRequest> :: 
+                && Message(pkt.src, pkt.dest, Spec.ParseServiceReply(pkt.msg).value) in v.multSvc.hosts[0].replies
                 && request in v.multSvc.hosts[0].requests 
                 && request.src == pkt.dest)
         && (forall request: Message<seq<byte>> ::
-            && Service.ParseServiceRequest(request.msg).Some?
-            && Message(request.src, request.dest, Service.ParseServiceRequest(request.msg).value) in v.multSvc.hosts[0].requests ==>
+            && Spec.ParseServiceRequest(request.msg).Some?
+            && Message(request.src, request.dest, Spec.ParseServiceRequest(request.msg).value) in v.multSvc.hosts[0].requests ==>
             && request in v.network.sentMsgs
             && request.dest == c.multSvc.hosts[0].idSelf)
     }
@@ -43,7 +43,7 @@ module RefinementProof refines RefinementTheorem {
     {
         && (forall pkt: Message<seq<byte>> ::
             && pkt in v.network.sentMsgs
-            && AddSvc.ParseServiceRequest(pkt.msg).Some?
+            && AddSM.ParseServiceRequest(pkt.msg).Some?
             && pkt.src == c.multSvc.hosts[0].idSelf ==>
                 Inv_MultSvcInductiveMultiplicationImpl(c, v, pkt))
     }
@@ -51,11 +51,11 @@ module RefinementProof refines RefinementTheorem {
     ghost predicate Inv_MultSvcInductiveMultiplicationImpl(c: Constants, v: Variables, pkt: Message<seq<byte>>)
         requires v.WF(c)
         requires pkt in v.network.sentMsgs
-        requires AddSvc.ParseServiceRequest(pkt.msg).Some?
+        requires AddSM.ParseServiceRequest(pkt.msg).Some?
         requires pkt.src == c.multSvc.hosts[0].idSelf
     {
         var vHost := v.multSvc.hosts[0];
-        var addReq := AddSvc.ParseServiceRequest(pkt.msg).value;
+        var addReq := AddSM.ParseServiceRequest(pkt.msg).value;
             && addReq.seqNo in vHost.seqNoAssgn
             && addReq.x == (addReq.seqNo - vHost.firstSeqNo[vHost.seqNoAssgn[addReq.seqNo]]) * vHost.seqNoAssgn[addReq.seqNo].msg.y
             && addReq.y == vHost.seqNoAssgn[addReq.seqNo].msg.y
@@ -69,13 +69,13 @@ module RefinementProof refines RefinementTheorem {
     {
         && (forall pkt: Message<seq<byte>> :: 
             && pkt in v.network.sentMsgs
-            && AddSvc.ParseServiceReply(pkt.msg).Some?
+            && AddSM.ParseServiceReply(pkt.msg).Some?
             && pkt.src == c.addSvc.idSelf ==>
                 exists req_pkt: Message<seq<byte>> :: 
                 && req_pkt in v.network.sentMsgs
-                && AddSvc.ParseServiceRequest(req_pkt.msg).Some?
-                && AddSvc.ParseServiceReply(pkt.msg).value.seqNo == AddSvc.ParseServiceRequest(req_pkt.msg).value.seqNo
-                && AddSvc.ParseServiceReply(pkt.msg).value.sum == AddSvc.ParseServiceRequest(req_pkt.msg).value.x + AddSvc.ParseServiceRequest(req_pkt.msg).value.y
+                && AddSM.ParseServiceRequest(req_pkt.msg).Some?
+                && AddSM.ParseServiceReply(pkt.msg).value.seqNo == AddSM.ParseServiceRequest(req_pkt.msg).value.seqNo
+                && AddSM.ParseServiceReply(pkt.msg).value.sum == AddSM.ParseServiceRequest(req_pkt.msg).value.x + AddSM.ParseServiceRequest(req_pkt.msg).value.y
                 && pkt.src == req_pkt.dest
                 && pkt.dest == req_pkt.src
         )
@@ -92,7 +92,7 @@ module RefinementProof refines RefinementTheorem {
     lemma RefinementInit(c: Constants, v: Variables)
         // requires Init(c, v)
         // ensures Inv(c, v)
-        // ensures Service.Init(ConstantsAbstraction(c), VariablesAbstraction(c, v))
+        // ensures Spec.Init(ConstantsAbstraction(c), VariablesAbstraction(c, v))
     {}
 
     lemma SetUnionHelper<T>(s1: set<T>, s2: set<T>, a: T, b: T)
@@ -105,26 +105,26 @@ module RefinementProof refines RefinementTheorem {
     lemma InvInductive_ReceiveRequestHelper(c: Constants, v: Variables, v': Variables, msgOps: MessageOps, recvPkt: Message<seq<byte>>, sendPkt: Message<seq<byte>>)
         requires Next(c, v, v', msgOps)
         requires Inv(c, v)
-        requires Service.ParseServiceRequest(recvPkt.msg).Some?
-        requires AddSvc.ParseServiceRequest(sendPkt.msg).Some?
-        requires MultSvc.Host.ReceiveRequestImpl(c.multSvc.hosts[0], v.multSvc.hosts[0], v'.multSvc.hosts[0], msgOps, recvPkt, sendPkt)
+        requires Spec.ParseServiceRequest(recvPkt.msg).Some?
+        requires AddSM.ParseServiceRequest(sendPkt.msg).Some?
+        requires MultSM.Host.ReceiveRequestImpl(c.multSvc.hosts[0], v.multSvc.hosts[0], v'.multSvc.hosts[0], msgOps, recvPkt, sendPkt)
         ensures Inv(c, v')
     {
         var cHost := c.multSvc.hosts[0];
         var vHost := v.multSvc.hosts[0];
         var v'Host := v'.multSvc.hosts[0];
-        var request := Message(recvPkt.src, recvPkt.dest, Service.ParseServiceRequest(recvPkt.msg).value);
-        var addRequest := Message(sendPkt.src, sendPkt.dest, AddSvc.ParseServiceRequest(sendPkt.msg).value);
+        var request := Message(recvPkt.src, recvPkt.dest, Spec.ParseServiceRequest(recvPkt.msg).value);
+        var addRequest := Message(sendPkt.src, sendPkt.dest, AddSM.ParseServiceRequest(sendPkt.msg).value);
         var addReq := addRequest.msg;
         assert sendPkt == Message(cHost.idSelf, cHost.idAdditionService, sendPkt.msg);
-        forall reqPkt: Message<seq<byte>> | Service.ParseServiceRequest(reqPkt.msg).Some? && Message(reqPkt.src, reqPkt.dest, Service.ParseServiceRequest(reqPkt.msg).value) in v'Host.requests
+        forall reqPkt: Message<seq<byte>> | Spec.ParseServiceRequest(reqPkt.msg).Some? && Message(reqPkt.src, reqPkt.dest, Spec.ParseServiceRequest(reqPkt.msg).value) in v'Host.requests
             ensures reqPkt in v'.network.sentMsgs && reqPkt.dest == cHost.idSelf
         {
-            if (Message(reqPkt.src, reqPkt.dest, Service.ParseServiceRequest(reqPkt.msg).value) !in vHost.requests) {
-                assert v'Host.requests == vHost.requests + {Message(recvPkt.src, recvPkt.dest, Service.ParseServiceRequest(recvPkt.msg).value)};
-                SetUnionHelper(vHost.requests, v'Host.requests, Message(recvPkt.src, recvPkt.dest, Service.ParseServiceRequest(recvPkt.msg).value), Message(reqPkt.src, reqPkt.dest, Service.ParseServiceRequest(reqPkt.msg).value));
-                assert Message(reqPkt.src, reqPkt.dest, Service.ParseServiceRequest(reqPkt.msg).value) == Message(recvPkt.src, recvPkt.dest, Service.ParseServiceRequest(recvPkt.msg).value);
-                Service.ParseOneToOne(reqPkt.msg, recvPkt.msg);
+            if (Message(reqPkt.src, reqPkt.dest, Spec.ParseServiceRequest(reqPkt.msg).value) !in vHost.requests) {
+                assert v'Host.requests == vHost.requests + {Message(recvPkt.src, recvPkt.dest, Spec.ParseServiceRequest(recvPkt.msg).value)};
+                SetUnionHelper(vHost.requests, v'Host.requests, Message(recvPkt.src, recvPkt.dest, Spec.ParseServiceRequest(recvPkt.msg).value), Message(reqPkt.src, reqPkt.dest, Spec.ParseServiceRequest(reqPkt.msg).value));
+                assert Message(reqPkt.src, reqPkt.dest, Spec.ParseServiceRequest(reqPkt.msg).value) == Message(recvPkt.src, recvPkt.dest, Spec.ParseServiceRequest(recvPkt.msg).value);
+                Spec.ParseOneToOne(reqPkt.msg, recvPkt.msg);
                 assert reqPkt == recvPkt;
             } else {
                 assert Inv_MultSvcCorrespondence(c, v);
@@ -142,7 +142,7 @@ module RefinementProof refines RefinementTheorem {
         assert addReq.seqNo == v'Host.firstSeqNo[v'Host.seqNoAssgn[addReq.seqNo]];
         assert addReq.x == 0;
         assert addReq.y == request.msg.y;
-        forall pkt | pkt in v'.network.sentMsgs && AddSvc.ParseServiceRequest(pkt.msg).Some? && pkt.src == c.multSvc.hosts[0].idSelf
+        forall pkt | pkt in v'.network.sentMsgs && AddSM.ParseServiceRequest(pkt.msg).Some? && pkt.src == c.multSvc.hosts[0].idSelf
             ensures Inv_MultSvcInductiveMultiplicationImpl(c, v', pkt)
         {
             if (pkt == sendPkt) {
@@ -150,7 +150,7 @@ module RefinementProof refines RefinementTheorem {
             } else {
                 assert pkt in v.network.sentMsgs;
                 assert Inv_MultSvcInductiveMultiplication(c, v);
-                var addReq := AddSvc.ParseServiceRequest(pkt.msg).value;
+                var addReq := AddSM.ParseServiceRequest(pkt.msg).value;
                 assert addReq.seqNo in v'Host.seqNoAssgn;
                 assert vHost.seqNoAssgn[addReq.seqNo] == v'Host.seqNoAssgn[addReq.seqNo];
                 assert vHost.firstSeqNo[vHost.seqNoAssgn[addReq.seqNo]] == v'Host.firstSeqNo[v'Host.seqNoAssgn[addReq.seqNo]];
@@ -169,16 +169,16 @@ module RefinementProof refines RefinementTheorem {
     lemma InvInductive_ReceiveIntermediateResponseHelper(c: Constants, v: Variables, v': Variables, msgOps: MessageOps, recvPkt: Message<seq<byte>>, sendPkt: Message<seq<byte>>) 
         requires Next(c, v, v', msgOps)
         requires Inv(c, v)
-        requires AddSvc.ParseServiceReply(recvPkt.msg).Some?
-        requires AddSvc.ParseServiceRequest(sendPkt.msg).Some?
-        requires MultSvc.Host.ReceiveIntermediateResponseImpl(c.multSvc.hosts[0], v.multSvc.hosts[0], v'.multSvc.hosts[0], msgOps, recvPkt, sendPkt)
+        requires AddSM.ParseServiceReply(recvPkt.msg).Some?
+        requires AddSM.ParseServiceRequest(sendPkt.msg).Some?
+        requires MultSM.Host.ReceiveIntermediateResponseImpl(c.multSvc.hosts[0], v.multSvc.hosts[0], v'.multSvc.hosts[0], msgOps, recvPkt, sendPkt)
         ensures Inv(c, v')
     {
         var cHost := c.multSvc.hosts[0];
         var vHost := v.multSvc.hosts[0];
         var v'Host := v'.multSvc.hosts[0];
-        var addReply := Message(recvPkt.src, recvPkt.dest, AddSvc.ParseServiceReply(recvPkt.msg).value);
-        var addRequest := Message(sendPkt.src, sendPkt.dest, AddSvc.ParseServiceRequest(sendPkt.msg).value);
+        var addReply := Message(recvPkt.src, recvPkt.dest, AddSM.ParseServiceReply(recvPkt.msg).value);
+        var addRequest := Message(sendPkt.src, sendPkt.dest, AddSM.ParseServiceRequest(sendPkt.msg).value);
         var addReq := addRequest.msg;
         assert sendPkt == Message(cHost.idSelf, cHost.idAdditionService, sendPkt.msg);
         UniqueParsingAxiom(sendPkt.msg);
@@ -191,14 +191,14 @@ module RefinementProof refines RefinementTheorem {
         assert addReply.msg.seqNo == vHost.firstSeqNo[request] + |vHost.intermediateResults[request]|;
         assert addReq.x == addReply.msg.sum;
         assert addReq.y == request.msg.y;
-        forall pkt | pkt in v'.network.sentMsgs && AddSvc.ParseServiceRequest(pkt.msg).Some? && pkt.src == c.multSvc.hosts[0].idSelf
+        forall pkt | pkt in v'.network.sentMsgs && AddSM.ParseServiceRequest(pkt.msg).Some? && pkt.src == c.multSvc.hosts[0].idSelf
             ensures Inv_MultSvcInductiveMultiplicationImpl(c, v', pkt)
         {
             if (pkt == sendPkt) {
-                var prevAddReq :| prevAddReq in v.network.sentMsgs && AddSvc.ParseServiceRequest(prevAddReq.msg).Some? && AddSvc.ParseServiceReply(recvPkt.msg).value.seqNo == AddSvc.ParseServiceRequest(prevAddReq.msg).value.seqNo && AddSvc.ParseServiceReply(recvPkt.msg).value.sum == AddSvc.ParseServiceRequest(prevAddReq.msg).value.x + AddSvc.ParseServiceRequest(prevAddReq.msg).value.y && recvPkt.src == prevAddReq.dest && recvPkt.dest == prevAddReq.src;
+                var prevAddReq :| prevAddReq in v.network.sentMsgs && AddSM.ParseServiceRequest(prevAddReq.msg).Some? && AddSM.ParseServiceReply(recvPkt.msg).value.seqNo == AddSM.ParseServiceRequest(prevAddReq.msg).value.seqNo && AddSM.ParseServiceReply(recvPkt.msg).value.sum == AddSM.ParseServiceRequest(prevAddReq.msg).value.x + AddSM.ParseServiceRequest(prevAddReq.msg).value.y && recvPkt.src == prevAddReq.dest && recvPkt.dest == prevAddReq.src;
                 assert prevAddReq.src == c.multSvc.hosts[0].idSelf;
                 assert Inv_MultSvcInductiveMultiplicationImpl(c, v, prevAddReq);
-                var prevAddReqParsed := AddSvc.ParseServiceRequest(prevAddReq.msg).value;
+                var prevAddReqParsed := AddSM.ParseServiceRequest(prevAddReq.msg).value;
                 assert prevAddReqParsed.seqNo == addReply.msg.seqNo;
                 assert prevAddReqParsed.seqNo + 1 == addReq.seqNo;
                 assert prevAddReqParsed.x == (prevAddReqParsed.seqNo - vHost.firstSeqNo[vHost.seqNoAssgn[prevAddReqParsed.seqNo]]) * vHost.seqNoAssgn[prevAddReqParsed.seqNo].msg.y && prevAddReqParsed.y == vHost.seqNoAssgn[prevAddReqParsed.seqNo].msg.y;
@@ -212,7 +212,7 @@ module RefinementProof refines RefinementTheorem {
             } else {
                 assert pkt in v.network.sentMsgs;
                 assert Inv_MultSvcInductiveMultiplication(c, v);
-                var addReq := AddSvc.ParseServiceRequest(pkt.msg).value;
+                var addReq := AddSM.ParseServiceRequest(pkt.msg).value;
                 assert addReq.seqNo in v'Host.seqNoAssgn;
                 assert vHost.seqNoAssgn[addReq.seqNo] == v'Host.seqNoAssgn[addReq.seqNo];
                 assert vHost.firstSeqNo[vHost.seqNoAssgn[addReq.seqNo]] == v'Host.firstSeqNo[v'Host.seqNoAssgn[addReq.seqNo]];
@@ -224,21 +224,21 @@ module RefinementProof refines RefinementTheorem {
     lemma InvInductive_ReceiveFinalResponseHelper(c: Constants, v: Variables, v': Variables, msgOps: MessageOps, recvPkt: Message<seq<byte>>, sendPkt: Message<seq<byte>>) 
         requires Next(c, v, v', msgOps)
         requires Inv(c, v)
-        requires AddSvc.ParseServiceReply(recvPkt.msg).Some?
-        requires Service.ParseServiceReply(sendPkt.msg).Some?
-        requires MultSvc.Host.ReceiveFinalResponseImpl(c.multSvc.hosts[0], v.multSvc.hosts[0], v'.multSvc.hosts[0], msgOps, recvPkt, sendPkt)
+        requires AddSM.ParseServiceReply(recvPkt.msg).Some?
+        requires Spec.ParseServiceReply(sendPkt.msg).Some?
+        requires MultSM.Host.ReceiveFinalResponseImpl(c.multSvc.hosts[0], v.multSvc.hosts[0], v'.multSvc.hosts[0], msgOps, recvPkt, sendPkt)
         ensures Inv(c, v')
     {
         var cHost := c.multSvc.hosts[0];
         var vHost := v.multSvc.hosts[0];
         var v'Host := v'.multSvc.hosts[0];
-        var addReply := Message(recvPkt.src, recvPkt.dest, AddSvc.ParseServiceReply(recvPkt.msg).value);
-        var reply := Message(sendPkt.src, sendPkt.dest, Service.ParseServiceReply(sendPkt.msg).value);
+        var addReply := Message(recvPkt.src, recvPkt.dest, AddSM.ParseServiceReply(recvPkt.msg).value);
+        var reply := Message(sendPkt.src, sendPkt.dest, Spec.ParseServiceReply(sendPkt.msg).value);
         assert sendPkt == Message(cHost.idSelf, vHost.seqNoAssgn[addReply.msg.seqNo].src, sendPkt.msg);
 
-        forall pkt: Message<seq<byte>> | pkt in v'.network.sentMsgs && Service.ParseServiceReply(pkt.msg).Some? && pkt.src == cHost.idSelf
-            ensures (exists request: Message<Service.ServiceRequest> :: 
-                && Message(pkt.src, pkt.dest, Service.ParseServiceReply(pkt.msg).value) in v'Host.replies
+        forall pkt: Message<seq<byte>> | pkt in v'.network.sentMsgs && Spec.ParseServiceReply(pkt.msg).Some? && pkt.src == cHost.idSelf
+            ensures (exists request: Message<Spec.ServiceRequest> :: 
+                && Message(pkt.src, pkt.dest, Spec.ParseServiceReply(pkt.msg).value) in v'Host.replies
                 && request in v'Host.requests 
                 && request.src == pkt.dest)
         {
@@ -266,44 +266,44 @@ module RefinementProof refines RefinementTheorem {
     {
         var step :| NextStep(c, v, v', msgOps, step);
         if (MultSvcAction(c, v, v', msgOps, step.hostId)) {
-            var hostStep :| MultSvc.NextStep(c.multSvc, v.multSvc, v'.multSvc, msgOps, hostStep);
+            var hostStep :| MultSM.NextStep(c.multSvc, v.multSvc, v'.multSvc, msgOps, hostStep);
             var cHost := c.multSvc.hosts[0];
             var vHost := v.multSvc.hosts[0];
             var v'Host := v'.multSvc.hosts[0];
-            assert MultSvc.Host.Next(cHost, vHost, v'Host, msgOps);
+            assert MultSM.Host.Next(cHost, vHost, v'Host, msgOps);
 
-            if (MultSvc.Host.ReceiveRequest(cHost, vHost, v'Host, msgOps)) {
-                var recvPkt: Message<seq<byte>>, sendPkt: Message<seq<byte>> :| Service.ParseServiceRequest(recvPkt.msg).Some? && AddSvc.ParseServiceRequest(sendPkt.msg).Some? && MultSvc.Host.ReceiveRequestImpl(cHost, vHost, v'Host, msgOps, recvPkt, sendPkt);
+            if (MultSM.Host.ReceiveRequest(cHost, vHost, v'Host, msgOps)) {
+                var recvPkt: Message<seq<byte>>, sendPkt: Message<seq<byte>> :| Spec.ParseServiceRequest(recvPkt.msg).Some? && AddSM.ParseServiceRequest(sendPkt.msg).Some? && MultSM.Host.ReceiveRequestImpl(cHost, vHost, v'Host, msgOps, recvPkt, sendPkt);
                 InvInductive_ReceiveRequestHelper(c, v, v', msgOps, recvPkt, sendPkt);
-            } else if (MultSvc.Host.ReceiveIntermediateResponse(cHost, vHost, v'Host, msgOps)) {
-                var recvPkt: Message<seq<byte>>, sendPkt: Message<seq<byte>> :| AddSvc.ParseServiceReply(recvPkt.msg).Some? && AddSvc.ParseServiceRequest(sendPkt.msg).Some? && MultSvc.Host.ReceiveIntermediateResponseImpl(cHost, vHost, v'Host, msgOps, recvPkt, sendPkt);
+            } else if (MultSM.Host.ReceiveIntermediateResponse(cHost, vHost, v'Host, msgOps)) {
+                var recvPkt: Message<seq<byte>>, sendPkt: Message<seq<byte>> :| AddSM.ParseServiceReply(recvPkt.msg).Some? && AddSM.ParseServiceRequest(sendPkt.msg).Some? && MultSM.Host.ReceiveIntermediateResponseImpl(cHost, vHost, v'Host, msgOps, recvPkt, sendPkt);
                 InvInductive_ReceiveIntermediateResponseHelper(c, v, v', msgOps, recvPkt, sendPkt);
             } else {
-                assert MultSvc.Host.ReceiveFinalResponse(cHost, vHost, v'Host, msgOps);
-                var recvPkt: Message<seq<byte>>, sendPkt: Message<seq<byte>>:| AddSvc.ParseServiceReply(recvPkt.msg).Some? && Service.ParseServiceReply(sendPkt.msg).Some? && MultSvc.Host.ReceiveFinalResponseImpl(cHost, vHost, v'Host, msgOps, recvPkt, sendPkt);
+                assert MultSM.Host.ReceiveFinalResponse(cHost, vHost, v'Host, msgOps);
+                var recvPkt: Message<seq<byte>>, sendPkt: Message<seq<byte>>:| AddSM.ParseServiceReply(recvPkt.msg).Some? && Spec.ParseServiceReply(sendPkt.msg).Some? && MultSM.Host.ReceiveFinalResponseImpl(cHost, vHost, v'Host, msgOps, recvPkt, sendPkt);
                 InvInductive_ReceiveFinalResponseHelper(c, v, v', msgOps, recvPkt, sendPkt);
             }
         } else {
             assert AddSvcAction(c, v, v', msgOps, step.hostId);
-            var recvPkt, sendPkt :| AddSvc.AddImpl(c.addSvc, v.addSvc, v'.addSvc, msgOps, recvPkt, sendPkt);
-            assert AddSvc.ParseServiceReply(sendPkt.msg).Some?;
-            assert AddSvc.ParseServiceRequest(recvPkt.msg).Some?;
+            var recvPkt, sendPkt :| AddSM.AddImpl(c.addSvc, v.addSvc, v'.addSvc, msgOps, recvPkt, sendPkt);
+            assert AddSM.ParseServiceReply(sendPkt.msg).Some?;
+            assert AddSM.ParseServiceRequest(recvPkt.msg).Some?;
 
             assert Inv_MultSvcCorrespondence(c, v');
             
-            forall pkt: Message<seq<byte>> | pkt in v'.network.sentMsgs && AddSvc.ParseServiceReply(pkt.msg).Some? && pkt.src == c.addSvc.idSelf
+            forall pkt: Message<seq<byte>> | pkt in v'.network.sentMsgs && AddSM.ParseServiceReply(pkt.msg).Some? && pkt.src == c.addSvc.idSelf
                 ensures (exists req_pkt: Message<seq<byte>> :: 
                 && req_pkt in v.network.sentMsgs
-                && AddSvc.ParseServiceRequest(req_pkt.msg).Some?
-                && AddSvc.ParseServiceReply(pkt.msg).value.seqNo == AddSvc.ParseServiceRequest(req_pkt.msg).value.seqNo
-                && AddSvc.ParseServiceReply(pkt.msg).value.sum == AddSvc.ParseServiceRequest(req_pkt.msg).value.x + AddSvc.ParseServiceRequest(req_pkt.msg).value.y
+                && AddSM.ParseServiceRequest(req_pkt.msg).Some?
+                && AddSM.ParseServiceReply(pkt.msg).value.seqNo == AddSM.ParseServiceRequest(req_pkt.msg).value.seqNo
+                && AddSM.ParseServiceReply(pkt.msg).value.sum == AddSM.ParseServiceRequest(req_pkt.msg).value.x + AddSM.ParseServiceRequest(req_pkt.msg).value.y
                 && pkt.src == req_pkt.dest
                 && pkt.dest == req_pkt.src)
             {
                 if (pkt == sendPkt) {
                     assert recvPkt in v'.network.sentMsgs;
-                    assert AddSvc.ParseServiceReply(pkt.msg).value.seqNo == AddSvc.ParseServiceRequest(recvPkt.msg).value.seqNo;
-                    assert AddSvc.ParseServiceReply(pkt.msg).value.sum == AddSvc.ParseServiceRequest(recvPkt.msg).value.x + AddSvc.ParseServiceRequest(recvPkt.msg).value.y;
+                    assert AddSM.ParseServiceReply(pkt.msg).value.seqNo == AddSM.ParseServiceRequest(recvPkt.msg).value.seqNo;
+                    assert AddSM.ParseServiceReply(pkt.msg).value.sum == AddSM.ParseServiceRequest(recvPkt.msg).value.x + AddSM.ParseServiceRequest(recvPkt.msg).value.y;
                 } else {
                     assert pkt in v.network.sentMsgs;
                 }
@@ -319,7 +319,7 @@ module RefinementProof refines RefinementTheorem {
         // requires Inv(c, v)
         // ensures Inv(c, v') 
         // ensures 
-        //     || Service.Next(ConstantsAbstraction(c), VariablesAbstraction(c, v), VariablesAbstraction(c, v'), MessageOps(ServiceRequestsAbstraction(msgOps.recv), ServiceRepliesAbstraction(msgOps.send)))
+        //     || Spec.Next(ConstantsAbstraction(c), VariablesAbstraction(c, v), VariablesAbstraction(c, v'), MessageOps(ServiceRequestsAbstraction(msgOps.recv), ServiceRepliesAbstraction(msgOps.send)))
         //     || (VariablesAbstraction(c, v) == VariablesAbstraction(c, v') && ServiceRequestsAbstraction(msgOps.recv) == {} && ServiceRepliesAbstraction(msgOps.send) == {})
     {
         InvInductive(c, v, v', msgOps);
@@ -330,37 +330,37 @@ module RefinementProof refines RefinementTheorem {
         var recvSvc := ServiceRequestsAbstraction(msgOps.recv);
         var sendSvc := ServiceRepliesAbstraction(msgOps.send);
         if (MultSvcAction(c, v, v', msgOps, step.hostId)) {
-            var hostStep :| MultSvc.NextStep(c.multSvc, v.multSvc, v'.multSvc, msgOps, hostStep);
+            var hostStep :| MultSM.NextStep(c.multSvc, v.multSvc, v'.multSvc, msgOps, hostStep);
             var cHost := c.multSvc.hosts[0];
             var vHost := v.multSvc.hosts[0];
             var v'Host := v'.multSvc.hosts[0];
-            assert MultSvc.Host.Next(cHost, vHost, v'Host, msgOps);
+            assert MultSM.Host.Next(cHost, vHost, v'Host, msgOps);
 
-            if (MultSvc.Host.ReceiveRequest(cHost, vHost, v'Host, msgOps)) {
-                var recvPkt: Message<seq<byte>>, sendPkt: Message<seq<byte>> :| Service.ParseServiceRequest(recvPkt.msg).Some? && AddSvc.ParseServiceRequest(sendPkt.msg).Some? && MultSvc.Host.ReceiveRequestImpl(cHost, vHost, v'Host, msgOps, recvPkt, sendPkt);
+            if (MultSM.Host.ReceiveRequest(cHost, vHost, v'Host, msgOps)) {
+                var recvPkt: Message<seq<byte>>, sendPkt: Message<seq<byte>> :| Spec.ParseServiceRequest(recvPkt.msg).Some? && AddSM.ParseServiceRequest(sendPkt.msg).Some? && MultSM.Host.ReceiveRequestImpl(cHost, vHost, v'Host, msgOps, recvPkt, sendPkt);
                 UniqueParsingAxiom(sendPkt.msg);
                 assert recvSvc == {recvPkt};
                 assert sendSvc == {};
-                assert Service.ReceiveRequest(cSvc, vSvc, v'Svc, MessageOps(recvSvc, sendSvc));
-            } else if (MultSvc.Host.ReceiveIntermediateResponse(cHost, vHost, v'Host, msgOps)) {
-                var recvPkt: Message<seq<byte>>, sendPkt: Message<seq<byte>> :| AddSvc.ParseServiceReply(recvPkt.msg).Some? && AddSvc.ParseServiceRequest(sendPkt.msg).Some? && MultSvc.Host.ReceiveIntermediateResponseImpl(cHost, vHost, v'Host, msgOps, recvPkt, sendPkt);
+                assert Spec.ReceiveRequest(cSvc, vSvc, v'Svc, MessageOps(recvSvc, sendSvc));
+            } else if (MultSM.Host.ReceiveIntermediateResponse(cHost, vHost, v'Host, msgOps)) {
+                var recvPkt: Message<seq<byte>>, sendPkt: Message<seq<byte>> :| AddSM.ParseServiceReply(recvPkt.msg).Some? && AddSM.ParseServiceRequest(sendPkt.msg).Some? && MultSM.Host.ReceiveIntermediateResponseImpl(cHost, vHost, v'Host, msgOps, recvPkt, sendPkt);
                 UniqueParsingAxiom(recvPkt.msg);
                 UniqueParsingAxiom(sendPkt.msg);
                 assert vSvc == v'Svc;
                 assert ServiceRequestsAbstraction(msgOps.recv) == {} && ServiceRepliesAbstraction(msgOps.send) == {};
             } else {
-                assert MultSvc.Host.ReceiveFinalResponse(cHost, vHost, v'Host, msgOps);
-                var recvPkt: Message<seq<byte>>, sendPkt: Message<seq<byte>>:| AddSvc.ParseServiceReply(recvPkt.msg).Some? && Service.ParseServiceReply(sendPkt.msg).Some? && MultSvc.Host.ReceiveFinalResponseImpl(cHost, vHost, v'Host, msgOps, recvPkt, sendPkt);
+                assert MultSM.Host.ReceiveFinalResponse(cHost, vHost, v'Host, msgOps);
+                var recvPkt: Message<seq<byte>>, sendPkt: Message<seq<byte>>:| AddSM.ParseServiceReply(recvPkt.msg).Some? && Spec.ParseServiceReply(sendPkt.msg).Some? && MultSM.Host.ReceiveFinalResponseImpl(cHost, vHost, v'Host, msgOps, recvPkt, sendPkt);
                 UniqueParsingAxiom(recvPkt.msg);
                 assert recvSvc == {};
                 assert sendSvc == {sendPkt};
 
-                var addReply := Message(recvPkt.src, recvPkt.dest, AddSvc.ParseServiceReply(recvPkt.msg).value);
-                var reply := Message(sendPkt.src, sendPkt.dest, Service.ParseServiceReply(sendPkt.msg).value);
-                var prevAddReq :| prevAddReq in v.network.sentMsgs && AddSvc.ParseServiceRequest(prevAddReq.msg).Some? && AddSvc.ParseServiceReply(recvPkt.msg).value.seqNo == AddSvc.ParseServiceRequest(prevAddReq.msg).value.seqNo && AddSvc.ParseServiceReply(recvPkt.msg).value.sum == AddSvc.ParseServiceRequest(prevAddReq.msg).value.x + AddSvc.ParseServiceRequest(prevAddReq.msg).value.y && recvPkt.src == prevAddReq.dest && recvPkt.dest == prevAddReq.src;
+                var addReply := Message(recvPkt.src, recvPkt.dest, AddSM.ParseServiceReply(recvPkt.msg).value);
+                var reply := Message(sendPkt.src, sendPkt.dest, Spec.ParseServiceReply(sendPkt.msg).value);
+                var prevAddReq :| prevAddReq in v.network.sentMsgs && AddSM.ParseServiceRequest(prevAddReq.msg).Some? && AddSM.ParseServiceReply(recvPkt.msg).value.seqNo == AddSM.ParseServiceRequest(prevAddReq.msg).value.seqNo && AddSM.ParseServiceReply(recvPkt.msg).value.sum == AddSM.ParseServiceRequest(prevAddReq.msg).value.x + AddSM.ParseServiceRequest(prevAddReq.msg).value.y && recvPkt.src == prevAddReq.dest && recvPkt.dest == prevAddReq.src;
                 assert prevAddReq.src == c.multSvc.hosts[0].idSelf;
                 assert Inv_MultSvcInductiveMultiplicationImpl(c, v, prevAddReq);
-                var prevAddReqParsed := AddSvc.ParseServiceRequest(prevAddReq.msg).value;
+                var prevAddReqParsed := AddSM.ParseServiceRequest(prevAddReq.msg).value;
                 assert prevAddReqParsed.seqNo == addReply.msg.seqNo;
                 assert prevAddReqParsed.x == (prevAddReqParsed.seqNo - vHost.firstSeqNo[vHost.seqNoAssgn[prevAddReqParsed.seqNo]]) * vHost.seqNoAssgn[prevAddReqParsed.seqNo].msg.y && prevAddReqParsed.y == vHost.seqNoAssgn[prevAddReqParsed.seqNo].msg.y;
                 assert addReply.msg.sum == (prevAddReqParsed.seqNo - vHost.firstSeqNo[vHost.seqNoAssgn[prevAddReqParsed.seqNo]]) * vHost.seqNoAssgn[prevAddReqParsed.seqNo].msg.y + vHost.seqNoAssgn[prevAddReqParsed.seqNo].msg.y;
@@ -371,16 +371,16 @@ module RefinementProof refines RefinementTheorem {
 
                 var request := vHost.seqNoAssgn[addReply.msg.seqNo];
                 assert request in vHost.requests;
-                assert reply.msg == Service.MultiplyReply(request.msg.seqNo, request.msg.x * request.msg.y);
+                assert reply.msg == Spec.MultiplyReply(request.msg.seqNo, request.msg.x * request.msg.y);
                 assert sendPkt.dest == request.src;
                 
-                assert Service.SendResponseImpl(cSvc, vSvc, v'Svc, MessageOps(recvSvc, sendSvc), request, sendPkt);
-                assert Service.SendResponse(cSvc, vSvc, v'Svc, MessageOps(recvSvc, sendSvc));
+                assert Spec.SendResponseImpl(cSvc, vSvc, v'Svc, MessageOps(recvSvc, sendSvc), request, sendPkt);
+                assert Spec.SendResponse(cSvc, vSvc, v'Svc, MessageOps(recvSvc, sendSvc));
             }
         } else {
             assert AddSvcAction(c, v, v', msgOps, step.hostId);
             assert vSvc == v'Svc;
-            var recv : Message<seq<byte>>, send : Message<seq<byte>> :| AddSvc.AddImpl(c.addSvc, v.addSvc, v'.addSvc, msgOps, recv, send);
+            var recv : Message<seq<byte>>, send : Message<seq<byte>> :| AddSM.AddImpl(c.addSvc, v.addSvc, v'.addSvc, msgOps, recv, send);
             UniqueParsingAxiom(recv.msg);
             UniqueParsingAxiom(send.msg);
             assert ServiceRequestsAbstraction(msgOps.recv) == {} && ServiceRepliesAbstraction(msgOps.send) == {};
