working/composition/event_based_refinement/load_balancer/service_correspondence/multiplication_service/MultiplicationDistributedSystemSM.v.dfy
@@ -1,0 +1,12 @@
+include "MultiplicationHost.v.dfy"
+include "../addition_service/AdditionServiceSM.t.dfy"
+include "../shared/AbstractNetwork.t.dfy"
+include "../shared/AbstractDistributedSystemSM.t.dfy"
+
+module Network refines AbstractNetwork {
+}
+
+module MultiplicationDistributedSystemSM refines AbstractDistributedSystemSM {
+    import opened Network = Network
+    import Host = MultiplicationHost
+}
